day8.thy
@@ -1,7 +1,7 @@
 section "Solution to Day 8 of AoC 2020"
 
 theory day8
-  imports Main "HOL.Code_Numeral" string_utils list_natural_utils natural_utils list_utils
+  imports Main "HOL.Code_Numeral" string_utils list_natural_utils natural_utils list_utils HOL.Option
 begin
 
 text "This is a solution to the puzzle for day 8"
@@ -9,7 +9,7 @@ text "This is a solution to the puzzle for day 8"
 subsection "Input parsing"
 
 datatype instr =
-  Nop
+  Nop integer
   |Acc integer
   |Jmp integer
 
@@ -18,7 +18,7 @@ type_synonym program = "instr list"
 definition parse_instr
   where "parse_instr s = (
     case hd s of
-      CHR ''n'' \<Rightarrow> Nop
+      CHR ''n'' \<Rightarrow> Nop (str_to_int (drop 4 s))
       |CHR ''j'' \<Rightarrow> Jmp (str_to_int (drop 4 s))
       |CHR ''a'' \<Rightarrow> Acc (str_to_int (drop 4 s))
   )"
@@ -37,7 +37,7 @@ subsection "Solution Algorithm"
 definition exec_instr :: "instr \<Rightarrow> integer \<Rightarrow> integer \<times> integer"
   where "exec_instr instr acc = (
     case instr of
-      Nop \<Rightarrow> (acc, 1)
+      Nop n \<Rightarrow> (acc, 1)
       | Acc n \<Rightarrow> (acc + n, 1)
       | Jmp n \<Rightarrow> (acc, n)
   )"
@@ -68,8 +68,48 @@ definition find_loop
 definition part1 :: "string \<Rightarrow> integer"
   where "part1 s = find_loop (parse_program (trim s))"
 
-definition part2 :: "string \<Rightarrow> natural"
-  where "part2 s = 0"
+fun fix_error
+  where "fix_error (Nop n) = (Jmp n)"
+  |"fix_error (Jmp n) = (Nop n)"
+  |"fix_error other = other"
+
+
+fun exec_program_to_exit :: "natural \<Rightarrow> _"
+  where
+    "exec_program_to_exit limit error_pc proglen p flags acc pc = (
+    if limit = 0 then undefined else (
+      if pc \<ge> proglen then
+        ((Some error_pc), acc)
+      else
+        if nth pc flags then
+          (None, acc)
+        else
+          (let (new_acc, pc_change) = (exec_instr (if (error_pc = pc) then (fix_error (nth pc p)) else (nth pc p)) acc) in
+            let new_flags = replace pc flags True in
+            exec_program_to_exit (limit - 1) error_pc proglen p new_flags new_acc (natural_of_integer ((integer_of_natural pc) + pc_change))
+          )
+        )
+      
+    )
+  "
+
+fun first_some :: "'a list \<Rightarrow> ('a \<Rightarrow> 'b option) \<Rightarrow> 'a option" where
+  "first_some [] f = None"
+  |"first_some (Cons h t) f = (if Option.is_none (f h) then first_some t f else Some h)"
+
+definition part2 :: "string \<Rightarrow> integer"
+  where "part2 s = (let program = parse_program (trim s) in
+    (let proglen = natural_len program in
+      (let flags = map (\<lambda> a . False) program in
+        (let result = first_some (map (\<lambda> n . exec_program_to_exit 9999 n proglen program flags 0 0) (naturals_to proglen)) (fst) in
+          (case (map_option (snd) result) of
+            None \<Rightarrow> 0
+            |Some (acc) \<Rightarrow> acc
+          )
+        )
+      )
+    )
+  )"
 
 subsection "Testing"
 
@@ -88,11 +128,9 @@ acc +6
 lemma "part1 example_input = 5"
   by eval
 
-lemma "part2 example_input = 0"
+lemma "part2 example_input = 8"
   by eval
 
-(* TODO remember to export part2 once complete *)
-
-export_code "part1" in Haskell module_name Solution
+export_code "part1" "part2" in Haskell module_name Solution
 
 end
